done

Capless/Inversion/Lookup.lean
@@ -10,53 +10,53 @@ def Store.lookup_inv_bound
   (hl : Store.Bound σ x v)
   (ht : TypedStore σ Γ)
   (hb : Context.Bound Γ x T) :
-  Typed Γ v (EType.type T) := by
+  ∃ Cv, Typed Γ v (EType.type T) Cv := by
   induction ht
   case empty => cases hb
   case val ih =>
     cases hl
     case here =>
       cases hb
-      rename_i E _ ht _ _
+      rename_i E _ _ ht _ _
       have ht1 := ht.weaken (T := E)
       simp [EType.weaken, EType.rename, CType.weaken] at *
-      exact ht1
+      constructor; exact ht1
     case there_val  =>
       have ⟨T1, hb1, heq⟩ := Context.var_bound_succ_inv hb
       subst heq
       rename_i hl _
-      have ih := ih hl hb1
-      rename_i E _ _ _ _ _ _ _
+      have ⟨Cv0, ih⟩ := ih hl hb1
+      rename_i E _ _ _ _ _ _ _ _
       have ih := ih.weaken (T := E)
       simp [EType.weaken, EType.rename, CType.weaken] at *
-      exact ih
+      constructor; exact ih
   case tval S _ ih =>
     cases hb; cases hl
     rename_i hb _ hl
-    have ih := ih hl hb
+    have ⟨Cv0, ih⟩ := ih hl hb
     have ih := ih.tweaken (b := TBinding.inst S)
     simp [EType.tweaken, EType.trename, CType.tweaken] at *
-    exact ih
+    constructor; exact ih
   case cval C _ ih =>
     cases hb; cases hl
     rename_i hb _ hl
-    have ih := ih hl hb
+    have ⟨Cv0, ih⟩ := ih hl hb
     have ih := ih.cweaken (b := CBinding.inst C)
     simp [EType.cweaken, EType.crename, CType.cweaken] at *
-    exact ih
+    constructor; exact ih
 
 theorem Store.lookup_inv_typing
   (hl : Store.Bound σ x v)
   (ht : TypedStore σ Γ)
-  (hx : Typed Γ (Term.var x) (EType.type (CType.capt C S))) :
-  ∃ Cv, Typed Γ v (EType.type (CType.capt Cv S)) := by
+  (hx : Typed Γ (Term.var x) (EType.type (CType.capt C S)) Cx) :
+  ∃ Cv Cv0, Typed Γ v (EType.type (CType.capt Cv S)) Cv0 := by
   have ⟨C0, S0, hb, hsub⟩ := Typed.var_inv hx
-  have hv := Store.lookup_inv_bound hl ht hb
+  have ⟨Cv0, hv⟩ := Store.lookup_inv_bound hl ht hb
   cases hsub
   rename_i hsc hss
-  constructor
+  constructor; constructor
   apply Typed.sub
-  exact hv
+  exact hv; apply Subcapt.refl
   constructor
   constructor
   apply Subcapt.refl
